fsFFI: encoding functions for ints as constant length byte arrays

basis/fsFFIScript.sml
@@ -148,6 +148,76 @@ val getNullTermStr_def = Define`
        else SOME(MAP (CHR o w2n) (TAKE sz bytes))
 `;
 
+(* encode/decode nums as 2 or 8 bytes *)
+(* similar to n2l & l2n but with padding *)
+val num_to_byte2_def = Define`
+  num_to_byte2 (i : num) : word8 list = [n2w (i DIV 256); n2w i]`
+
+val num_to_byte8_def = Define`
+  num_to_byte8 (i : num) : word8 list =
+   [n2w (i DIV 256**7); n2w (i DIV 256**6);
+    n2w (i DIV 256**5); n2w (i DIV 256**4);
+    n2w (i DIV 256**3); n2w (i DIV 256**2);
+    n2w (i DIV 256); n2w i]`
+
+val byte2_to_num_def = Define`
+  byte2_to_num ([b1; b0] : word8 list) = w2n b1 * 256 + w2n b0`
+
+val byte8_to_num_def = Define`
+  byte8_to_num ([b7; b6; b5; b4; b3; b2; b1; b0] : word8 list) =
+  256 * ( 256 * ( 256 * ( 256 * ( 256 * ( 256 * ( 256 *
+  w2n b7 + w2n b6) + w2n b5) + w2n b4) + w2n b3) + w2n b2) + w2n b1) + w2n b0`
+
+val b2n_nb2 = Q.store_thm("b2n_nb2",
+  `!i. i < 2**(2*8) ==> byte2_to_num (num_to_byte2 i) = i`,
+  rw[byte2_to_num_def,num_to_byte2_def] >>
+  `0 < (256 : num)` by fs[] >> imp_res_tac DIVISION >> fs[] >>
+  first_x_assum (assume_tac o Q.SPEC`i`) >> fs[]);
+
+val nb2_b2n = Q.store_thm("nb2_b2n",
+  `!b. LENGTH b = 2 ==> num_to_byte2 (byte2_to_num b) = b`,
+  Cases_on`b` >> fs[] >> Cases_on`t` >> rw[byte2_to_num_def,num_to_byte2_def]
+  >-(PURE_REWRITE_TAC[Once MULT_COMM] >> fs[ADD_DIV_ADD_DIV] >>
+     fs[LESS_DIV_EQ_ZERO,w2n_lt_256]) >>
+  fs[GSYM word_add_n2w,GSYM word_mul_n2w] >>
+  `256w : word8 = 0w` by fs[GSYM n2w_dimword] >>
+  first_x_assum (fn x => PURE_REWRITE_TAC[x]) >> fs[]);
+
+val b8n_nb8 = Q.store_thm("b8n_nb8",
+  `!i. i <= 256**8 - 1 ==> byte8_to_num (num_to_byte8 i) = i`,
+  rw[byte8_to_num_def,num_to_byte8_def] >>
+  `0 < (256 : num)` by fs[] >> imp_res_tac DIVISION >> fs[] >> rw[] >>
+  NTAC 6(qmatch_abbrev_tac`256* i0 + x MOD 256 = x` >>
+      `i0 = x DIV 256` suffices_by fs[] >>
+      unabbrev_all_tac >> fs[DIV_DIV_DIV_MULT]) >>
+  PURE_REWRITE_TAC[Once ADD_COMM] >>
+  qmatch_abbrev_tac`256* i0 + x MOD 256 = x` >>
+  `i0 = x DIV 256` suffices_by fs[] >>
+  unabbrev_all_tac >> fs[DIV_DIV_DIV_MULT] >>
+  `i DIV 256**7 <= 255` suffices_by fs[] >>
+  fs[DIV_LE_X]);
+
+
+val nb8_b8n = Q.store_thm("nb8_nb8",
+  `!b. LENGTH b = 8 ==> num_to_byte8 (byte8_to_num b) = b`,
+  Cases_on`b` >> fs[] >>
+  NTAC 4 (Cases_on`t` >> fs[] >> Cases_on`t'` >> fs[]) >>
+  fs[byte8_to_num_def,num_to_byte8_def] >> rpt (TRY strip_tac
+  >-(rpt(qmatch_goalsub_abbrev_tac`(a + 256 * b) DIV m` >>
+         `m = 256 * (m DIV 256)` by fs[Abbr`m`] >>
+         first_x_assum (fn x => PURE_REWRITE_TAC[Once x]) >>
+         `0 < m DIV 256` by fs[Abbr`m`] >>
+         fs[GSYM DIV_DIV_DIV_MULT] >>
+         `0 < 256 : num` by fs[] >> imp_res_tac ADD_DIV_ADD_DIV >>
+         fs[] >>
+         unabbrev_all_tac >> rw[LESS_DIV_EQ_ZERO,w2n_lt_256]) >>
+     PURE_REWRITE_TAC[Once ADD_COMM] >>
+     TRY (first_x_assum(fn x => PURE_REWRITE_TAC[x])) >>
+     rw[LESS_DIV_EQ_ZERO,w2n_lt_256] >>
+     fs[GSYM word_add_n2w,GSYM word_mul_n2w] >>
+     `256w : word8 = 0w` by fs[GSYM n2w_dimword] >>
+     first_x_assum (fn x => PURE_REWRITE_TAC[x]) >> fs[])));
+
 (* read file name from the first non null bytes
 *  open the file with read access
 *  return result code in first byte
